Implementation/Lean/Cpn2mCrl2.lean
@@ -9,5 +9,6 @@ import Cpn2mCrl2.Semantics
 import Cpn2mCrl2.Lpe
 import Cpn2mCrl2.Translate
 import Cpn2mCrl2.Correct
+import Cpn2mCrl2.ListEncoding
 import Cpn2mCrl2.Print
 import Cpn2mCrl2.Json
