Implementation/Lean/Cpn2mCrl2/Typing.lean
@@ -95,15 +95,10 @@ theorem eval_wf : ∀ {τ : ExprTy} (e : Expr τ) {env : Env}, env.WfOn e.freeVa
       show ((eval a _ ++ eval b _).all fun v => v.ofColor _) = true
       simp only [List.all_append, Bool.and_eq_true]
       exact ⟨ha, hb⟩
-  | _, .rmList e l, _, h => by
-      have hl := eval_wf l fun p hp => h p (List.mem_append_right _ hp)
-      show ((eraseFirst (eval l _) (eval e _)).all fun v => v.ofColor _) = true
-      exact List.all_eq_true.2 fun v hv => List.all_eq_true.1 hl v (mem_of_mem_eraseFirst hv)
   | _, .diffList a b, _, h => by
       have ha := eval_wf a fun p hp => h p (List.mem_append_left _ hp)
       show ((listDiff (eval a _) (eval b _)).all fun v => v.ofColor _) = true
       exact List.all_eq_true.2 fun v hv => List.all_eq_true.1 ha v (mem_of_mem_listDiff hv)
-  | _, .inList _ _, _, _ => rfl
   | _, .subList _ _, _, _ => rfl
   | _, .bagDiff a b, _, h => by
       have ha := eval_wf a fun p hp => h p (List.mem_append_left _ hp)
